\documentclass[%
  hwnumber=6,%
  studentnumber=20053722,%
  {name=Bryan Hoang}%
]{%
  mthe353answer%
}

\begin{document}
  \begin{questions}
    \setcounter{question}{0}
    \question{}
    \begin{solution}
      \begin{proof}
        To prove the equality, we shall start with the RHS\@.
        \begin{align*}
          \text{RHS} &= \E{\cov(X_1, X_2)|Y} + \cov(\E{X_1|Y}, \E{X_2|Y})\\
          \begin{split}
            &= \E{\E{X_1 X_1|Y} - \E{X_1|Y}\E{X_2|Y}} + \E{\E{X_1|Y}\E{X_2|Y}}\\
            & \phantom{{}={}} - \E{\E{X_1|Y}}\E{\E{X_2|Y}}
          \end{split}\\
          &= \E{\E{X_1 X_1|Y}} - \E{\E{X_1|Y}\E{X_2|Y}}
            + \E{\E{X_1|Y}\E{X_2|Y}} - \E{X_1}\E{X_2}
          \shortintertext{by the linearity of expectation and the law of total expectation}
          &= \E{X_1 X_1} - \E{X_1}\E{X_2}
          \shortintertext{by the law of total expectation}
          &= \cov(X_1 X_2)\\
          &= \text{LHS} \qedhere
        \end{align*}
      \end{proof}
    \end{solution}
  \end{questions}
\end{document}
