\documentclass{mthe353answer}

\lhead{
  MTHE/STAT 353 - Homework 2, 2020\\
  \vspace{1em}
  \underline{\makebox[1.35in][c]{20053722}}\\
  Student Number
}

\begin{document}
  \begin{questions}
    \setcounter{question}{1}
    \question{}
    \begin{align*}
      E[X_1^2X_2^2 \dots X_n^2] =&\; E[X_1^2] \dots E[X_n^2] && \because X_1, \dots, X_n \text{ are independent}\\
      =& \int_{-\infty}^{\infty} x_1^2 f(x_1) \, \mathrm{d}x_1\; \dots \int_{-\infty}^{\infty} x_n^2 f(x_n) \, \mathrm{d}x_n && \text{by LOTUS}\\
      =& \int_{0}^{\infty} \frac{3x_1^2}{(x_1+1)^4} \, \mathrm{d}x_1\; \dots \int_{0}^{\infty} \frac{3x_n^2}{(x_n+1)^4} \, \mathrm{d}x_n
    \end{align*}
    Let \(I_i = \int_{0}^{\infty} \frac{3x_i^2}{(x_i+1)^4} \, \mathrm{d}x_i\).
    To evaluate \(I_i\), let's apply partial fraction decomposition to its
    integrand.
    \begin{align*}
      \frac{3x_i^2}{(x_i+1)^4} =&\; \frac{A}{x_i+1} + \frac{B}{(x_i+1)^2} + \frac{C}{(x_i+1)^3} + \frac{D}{(x_i+1)^4}\\
      =&\; \frac{A(x_i+1)^3 + B(x_i+1)^2 + C(x_i+1)^1 + D}{(x_i+1)^4}\\
      3x_i^2 =&\; A(x_i+1)^3 + B(x_i+1)^2 + C(x_i+1)^1 + D\\
      =&\; Ax_i^3 + (3A + B)x_i^2 + (3A + 2B + C)x_i + A + B + C + D\\
      \Rightarrow& \left\{
        \begin{aligned}
          A + B + C + D =&\; 0\\
          3A + 2B + C =&\; 0\\
          3A + B =&\; 3\\
          A =&\; 0
        \end{aligned}
      \right.\\
      \Rightarrow& \begin{augmentedmatrix}{4}
        1 & 1 & 1 & 1 & 0\\
        3 & 2 & 1 & 0 & 0\\
        3 & 1 & 0 & 0 & 3\\
        1 & 0 & 0 & 0 & 0
      \end{augmentedmatrix}\\
      \Rightarrow& \begin{augmentedmatrix}{4}
        1 & 0 & 0 & 0 & 0\\
        0 & 1 & 0 & 0 & 3\\
        0 & 0 & 1 & 0 & -6\\
        0 & 0 & 0 & 1 & 3
      \end{augmentedmatrix}\\
      \Rightarrow& \left\{
        \begin{aligned}
          A =&\; 0\\
          B =&\; 3\\
          C =&\; {-6}\\
          D =&\; 3
        \end{aligned}
      \right.\\
      \Rightarrow \frac{3x_i^2}{(x_i+1)^4} =&\; \frac{3}{(x_i+1)^2} - \frac{6}{(x_i+1)^3} + \frac{3}{(x_i+1)^4}
    \end{align*}
    Therefore,
    \begin{align*}
      I_i =& \int_{0}^{\infty} \frac{3}{(x_i+1)^2} - \frac{6}{(x_i+1)^3} + \frac{3}{(x_i+1)^4} \, \mathrm{d}x_i\\
      =& \left[-\frac{3}{(x_i+1)} + \frac{3}{(x_i+1)^2} - \frac{1}{(x_i+1)^3}\right]_{x_i=0}^{x_i=\infty}\\
      =& \frac{3}{(0+1)} - \frac{3}{(0+1)^2} + \frac{1}{(0+1)^3}\\
      =& 1, \quad \forall i \in \{1, \dots, n\}
    \end{align*}
    Hence,
    \begin{align*}
      E[X_1^2X_2^2 \dots X_n^2] =&\; 1 \times \cdots \times 1\\
      \alignedbox{=}{1}
    \end{align*}
  \end{questions}
\end{document}
