\documentclass[hwnumber=3]{mthe353answer}

\begin{document}
  \begin{questions}
    \setcounter{question}{4}
    \question{}
    Showing that~\eqref{eq:toprove} is true.
    \begin{equation}
      \label{eq:toprove}
      \lim\limits_{n \rightarrow \infty} P(X_{(n)} - \ln n \le x) = \exp(-e^{-x})
    \end{equation}
    \begin{solution}
      \begin{proof}
        Since the mean of each \(X_i,\; i \in \{1, \dots, n\}\), is 1, that means
        \(\lambda = 1\). Given the premise, the pdf of \(X_(n)\) is
        \begin{align*}
          f_n(x) &= nf(x)F(x)^{n-1}
          \shortintertext{Then the cdf of \(X_(n)\) is}
          F_n(x) &= \int_{\infty}^x nf(x)F(x)^{n-1} \dd{x_n}\\
          &= F(x)^n
          \shortintertext{where \(F(x)\) is the common cdf of the \(X_i\)}
        \end{align*}
        Hence, the LHS of~\eqref{eq:toprove} is
        \begin{align*}
          \limit{n}{\infty} P(X_{(n)} - \ln n \le x) &= \limit{n}{\infty} P(X_{(n)} \le x + \ln n)\\
          &= \limit{n}{\infty} F_n(x + \ln n)\\
          &= \limit{n}{\infty} F(x + \ln n)^n\\
          &= \limit{n}{\infty} (1 - e^{-(x + \ln n)})^n\\
          &= \limit{n}{\infty} \left(1 + \frac{(-e^{-x})}{n}\right)^n\\
          &= \exp(-e^{-x})\\
          &= \text{RHS of~\eqref{eq:toprove}}\qedhere
        \end{align*}
      \end{proof}
    \end{solution}
  \end{questions}
\end{document}
