\documentclass[hwnumber=5,studentnumber=20053722]{mthe353answer}

\begin{document}
  \begin{questions}
    \setcounter{question}{2}
    \question{}
    A fair coin is tossed successively. Let \(K_n\) be the number of tosses until
    \(n\) consecutive heads occur. Find \(\expect{K_n}\) for \(n \in \integers_{\ge} 1\).
    Hint: Condition on \(K_{n-1}\) and use the boundary condition \(\expect{K_1}=2\).
    \begin{solution}
      Looking at \(\expect{K_n|K_{n-1}=k}\), for \(k \in \integers_{\ge 1}\),
      we have two equally likely cases on the \(k\)th flip:
      \begin{itemize}
        \item If the \(k+1\) flip is heads, we are done. So the expected number
          is \(k + 1\)
        \item If the \(k+1\) flip is tails, we `start over'. So the expected
          number is \(k + 1 + \expect{K_n}\)
      \end{itemize}
      Thus, \(\expect{K_n|K_{n-1}=k} = \frac{1}{2}(k+1) + \frac{1}{2}(k+1+\expect{K_n})\).

      It follows that
      \begin{align*}
        \expect{K_n|K_{n-1}} &= \frac{1}{2}(K_{n-1}+1) +
          \frac{1}{2}(K_{n-1}+1+\expect{K_n})\\
        &= K_{n-1} + 1 + \frac{1}{2}\expect{K_n}
      \end{align*}
      By the law of total expectation, we have
      \begin{align*}
        \expect{K_n} &= \expect{\expect{K_n|K_{n-1}}}\\
        &= \expect{K_{n-1} + 1 + \frac{1}{2}\expect{K_n}}\\
        &= \expect{K_{n-1}} + 1 + \frac{1}{2}\expect{K_n}
      \end{align*}
      which implies the recurrence relation \(\expect{K_n} = 2\expect{K_{n-1}} + 2\).

      Solving the recurrence relation:
      \begin{align*}
        \expect{K_n} &= 2^1\expect{K_{n-1}} + 2(2^0)\\
        &= 2^1(2\expect{K_{n-2}} + 2) + 2(2^0)\\
        &= 2^2\expect{K_{n-2}} + 2(2^0 + 2^1)\\
        &= 2^2(2\expect{K_{n-3}} +2) + 2(2^0 + 2^1)\\
        &= 2^3\expect{K_{n-3}} + 2(2^0 + 2^1 + 2^2)\\
        &\phantom{{}={}}\vdots\\
        &= 2^m\expect{K_{n-m}} + 2\sum_{i=0}^{m-1} 2^i\\
        &= 2^m\expect{K_{n-m}} + 2\left(\frac{2^m-1}{2-1}\right)\\
        &= 2^m\expect{K_{n-m}} + 2^{m+1}-2\\
        &\phantom{{}={}}\vdots\\
        &= 2^{n-1}\expect{K_{n-(n-1)}} + 2^{(n-1)+1} - 2\\
        &= 2^{n-1}\expect{K_{1}} + 2^{n} - 2\\
        &= 2^{n-1}(2) + 2^{n} - 2\\
        &= 2^{n-1}(2) + 2^{n} - 2\\
        \alignedbox{= 2^{n+1} - 2, \quad \forall n \in \integers_{\ge 1}}
      \end{align*}
    \end{solution}
  \end{questions}
\end{document}
